Tests/testContract.fsx
@@ -1,0 +1,18 @@
+#I "bin"
+#r "Compile.Test.dll"
+#I "../bin/Debug/"
+#r "Consensus.dll"
+#r "Zulib.dll"
+#r "System.Reflection.Metadata.dll"
+#r "FSharp.Compatibility.OCaml.dll"
+#r "mscorlib.dll"
+#r "System.Core.dll"
+#r "System.dll"
+#r "System.Numerics.dll"
+
+open Compile.Test
+open Zen.Types.Extracted
+
+type Nonce = nonce
+
+let contractMain = mainFunction
